src/program_proof/session/canApply/proof.v
@@ -1,0 +1,82 @@
+From Goose.github_com.session Require Import canApply.
+From Perennial.program_proof Require Import std_proof. 
+From Perennial.goose_lang.ffi.grove_ffi Require Export impl.
+From Perennial.program_logic Require Export atomic.
+From Perennial.program_proof Require Export proof_prelude.
+From Perennial.program_proof Require Import grove_prelude.
+From Perennial.goose_lang.lib Require Import struct.struct into_val.
+From RecordUpdate Require Import RecordSet.
+From Perennial.goose_lang Require Import prelude.
+
+Local Lemma Z_scope_test : (0%Z) + (0%Z) = 0%Z.
+Proof. done. Qed.
+
+Section heap.
+  
+  Context `{hG: !heapGS Σ}.
+
+  Fixpoint coqCanApply (serverId: w64) (v1: list w64) (v2: list w64) (index: nat) (canApply: bool) : bool :=
+    match v1 with
+    | [] => true
+    | cons h1 t1 => match v2 with
+                    | [] => true
+                    | cons h2 t2 => if (uint.nat serverId) =? index then
+                                      (coqCanApply serverId t1 t2 (index + 1) (canApply))
+                                      else (if (canApply && (uint.Z h1 + 1 =? uint.Z h2)) then (coqCanApply serverId t1 t2 (index + 1) (false)) else false)
+                    end
+    end.
+                      
+  Lemma canApply_equiv (serverId: w64) (x: Slice.t) (xs: list w64) (y: Slice.t) (ys: list w64) :
+    {{{
+          own_slice x uint64T (DfracOwn 1) xs ∗
+          own_slice y uint64T (DfracOwn 1) ys ∗
+          ⌜length xs = length ys⌝ ∗
+          ⌜length xs < 2^64⌝
+    }}}
+       oneOffVersionVector #serverId x y 
+      {{{
+            r , RET #r;
+            ⌜r = coqCanApply serverId xs ys 0 true⌝ ∗ 
+            own_slice x uint64T (DfracOwn 1) xs ∗
+            own_slice y uint64T (DfracOwn 1) ys ∗
+            ⌜length xs = length ys⌝ ∗
+            ⌜length xs < 2^64⌝
+      }}}.
+  Proof.
+    iIntros (Φ) "(H1 & H2 & H3 & H4) H5".
+    unfold oneOffVersionVector. wp_pures.
+    wp_apply wp_ref_to; auto.
+    iIntros (output) "H6". wp_pures.
+    wp_apply wp_ref_to; auto.
+    iIntros (canApply) "H7". wp_pures.
+    wp_apply wp_ref_to; auto.
+    iIntros (index) "H8". wp_pures.
+    wp_apply wp_slice_len.
+    wp_apply wp_ref_to; auto.
+    iIntros (l) "H9". wp_pures.
+    wp_apply (wp_forBreak_cond
+                (λ continue,
+                  ∃ (b1 b2: bool) (i: w64),
+                    "Hx" ∷ own_slice x uint64T (DfracOwn 1) xs ∗
+                      "Hy" ∷ own_slice y uint64T (DfracOwn 1) ys ∗
+                      output ↦[boolT] #b1 ∗
+                      canApply ↦[boolT] #b2 ∗
+                      index ↦[uint64T] #i ∗
+                      l ↦[uint64T] #(length xs) 
+                )%I
+               with "[] []").
+    - iIntros (?). iModIntro. iIntros "H1 H2".
+      iNamed "H1". iDestruct "H1" as "(H1 & H3 & H4 & H5)".
+      wp_load. wp_load. wp_if_destruct.
+      + wp_load. wp_if_destruct.
+        * wp_load. wp_pures. wp_store. iModIntro. iApply "H2".
+          iExists (b1). iExists (b2).
+          iExists ((w64_word_instance.(word.add) serverId (W64 1))).
+          iFrame.
+        * 
+
+
+    
+
+
+
